proof using termination of the computation & admiting lifting lemma

theories/trans.v
@@ -387,30 +387,31 @@ Then, [trans_cont] would be simply be [map_cont trans_term trans_value] and [tra
 This is mostly the case, except for the default related continuations.
 *)
 
-Fixpoint trans_conts (kappa: list cont) : list cont :=
+Fixpoint trans_conts (kappa: list cont) (sigma: list value): list cont :=
   match kappa with
   | nil => nil
-  | CAppR t2 :: kappa => CAppR (trans t2) :: trans_conts kappa
-  | CBinopL op v1 :: kappa => CBinopL op (trans_value v1) :: trans_conts kappa
-  | CBinopR op t2 :: kappa => CBinopR op (trans t2) :: trans_conts kappa
-  | CClosure t_cl sigma_cl :: kappa => CClosure (trans t_cl) (List.map trans_value sigma_cl) :: trans_conts kappa
-  | CReturn sigma' :: kappa => CReturn (List.map trans_value sigma') :: trans_conts kappa
-  | CDefaultBase tc :: kappa => CIf (trans tc) ENone :: trans_conts kappa
-  | CMatch t1 t2 :: kappa => CMatch (trans t1) (trans t2) :: trans_conts kappa
-  | CSome :: kappa => CSome :: trans_conts kappa
-  | CIf t1 t2 :: kappa => CIf (trans t1) (trans t2) :: trans_conts kappa
-  | CErrorOnEmpty :: kappa => CMatch Conflict (Var 0) :: trans_conts kappa
-  | CDefaultPure :: kappa => CSome :: trans_conts kappa
+  | CAppR t2 :: kappa => CAppR (trans t2) :: trans_conts kappa sigma
+  | CBinopL op v1 :: kappa => CBinopL op (trans_value v1) :: trans_conts kappa sigma
+  | CBinopR op t2 :: kappa => CBinopR op (trans t2) :: trans_conts kappa sigma
+  | CClosure t_cl sigma_cl :: kappa => CClosure (trans t_cl) (List.map trans_value sigma_cl) :: trans_conts kappa sigma
+  | CReturn sigma' :: kappa => CReturn (List.map trans_value sigma') :: trans_conts kappa (List.map trans_value sigma')
+  | CDefaultBase tc :: kappa => CIf (trans tc) ENone :: trans_conts kappa sigma
+  | CMatch t1 t2 :: kappa => CMatch (trans t1) (trans t2) :: trans_conts kappa sigma
+  | CSome :: kappa => CSome :: trans_conts kappa sigma
+  | CIf t1 t2 :: kappa => CIf (trans t1) (trans t2) :: trans_conts kappa sigma
+  | CErrorOnEmpty :: kappa => CMatch Conflict (Var 0) :: trans_conts kappa sigma
+  | CDefaultPure :: kappa => CSome :: trans_conts kappa sigma
   | CDefault b None ts tj tc :: kappa =>
-    CMatch (monad_handle_zero (List.map trans ts) (trans tj) (trans tc)) (monad_handle_one (Var 0) (List.map trans ts)) :: trans_conts kappa
+    CMatch (monad_handle_zero (List.map trans ts) (trans tj) (trans tc)) (monad_handle_one (Var 0) (List.map trans ts)) :: trans_conts kappa sigma
 
   | CDefault b (Some v) ts tj tc :: kappa =>
+    CReturn (trans_value v::sigma) ::
     CMatch (
-      monad_handle_one'
-        (Value (trans_value v))
+      monad_handle_one
+        (Var 0)
         (List.map trans ts)
       )
-      (Conflict) :: trans_conts kappa
+      (Conflict) :: CReturn sigma :: trans_conts kappa sigma
 
   end.
 
@@ -424,9 +425,9 @@ Definition trans_return (r: result): result:=
 Definition trans_state (s: state) : state :=
   match s with
   | mode_eval e kappa env =>
-    mode_eval (trans e) (trans_conts kappa) (List.map trans_value env)
+    mode_eval (trans e) (trans_conts kappa (List.map trans_value env)) (List.map trans_value env)
   | mode_cont kappa env r =>
-    mode_cont (trans_conts kappa) (List.map trans_value env) (trans_return r)
+    mode_cont (trans_conts kappa (List.map trans_value env)) (List.map trans_value env) (trans_return r)
   end
 .
 
@@ -434,6 +435,20 @@ Definition trans_state (s: state) : state :=
 (* Require Import simulation_sred_to_cred. *)
 
 Import List.ListNotations.
+
+(* Lemma lift_cred:
+forall v e ts sigma, exists target,
+  star cred
+    (mode_eval (lift 1 e) [CMatch (monad_handle_one (Var 0) ts) Conflict; CReturn sigma] (v :: sigma))
+    target
+  /\
+  star cred
+    (mode_eval e [CMatch (monad_handle_one' (Value v) ts) Conflict] sigma)
+    target.
+Proof.
+
+Admitted.
+
 
 Lemma thing: forall ts sigma v GGamma Gamma T,
   List.Forall (fun ti : term => jt_term GGamma Gamma ti (TDefault T)) ts ->
@@ -449,12 +464,56 @@ Proof.
   intros.
   induction ts; simpl; unpack.
   { repeat step; eapply diagram_finish. }
-  { repeat step. 
-    admit.
+  { repeat step.
+    edestruct (lift_cred (trans_value v) (trans a) (List.map trans ts) (List.map trans_value sigma)) as (target1 & Ht1 & Ht2).
+    exists target1; eauto.
   }
-Admitted.
+Qed. *)
 
 Require Import sequences.
+
+Lemma append_stack_nil_eval:
+  forall {t kappa sigma},
+    mode_eval t kappa sigma = append_stack (mode_eval t [] sigma) kappa.
+Proof.
+  intros; simpl; eauto.
+Qed.
+
+Lemma append_stack_nil_cont:
+  forall {kappa sigma r},
+    mode_cont kappa sigma r = append_stack (mode_cont [] sigma r) kappa.
+Proof.
+  intros; simpl; eauto.
+Qed.
+
+Lemma thing:
+  forall {t sigma sigma' r a},
+  star cred (mode_eval t [] sigma) (mode_cont [] sigma' r ) ->
+  star cred (mode_eval (lift 1 t) [] (a :: sigma)) (mode_cont [] (a:: sigma') r).
+Admitted.
+
+Require Import simulation_sred_to_cred.
+
+Lemma cred_last:
+  forall s1 s2,
+    cred s1 s2 ->
+    last (stack s1) (env s1) = last (stack s2) (env s2).
+Proof.
+  induction 1; try induction phi; simpl; eauto.
+  { exfalso. eapply H; eauto. }
+Qed.
+
+Lemma star_cred_last:
+  forall s1 s2,
+    star cred s1 s2 ->
+    last (stack s1) (env s1) = last (stack s2) (env s2).
+Proof.
+  induction 1 as [|? ? ? Hstep Hstar].
+  { eauto. }
+  { pose proof (cred_last _ _ Hstep).
+    rewrite H; eauto.
+  }
+Qed.
 
 Theorem correction_continuations:
   forall s1 s2,
@@ -485,23 +544,44 @@ Proof.
     destruct h
   end.
 
-  all: try induction phi; try induction o;
+  all: try induction phi; try induction o.
+  all:
     try solve [simpl; repeat step; tryfalse; try eapply diagram_finish; eauto].
   {
     eexists; split; asimpl; [|eapply star_refl].
-    eapply star_one; simpl; econstructor; eauto using List.map_nth_error.
+    eapply star_one; simpl; econstructor. eauto using List.map_nth_error.
   }
-  { simpl.
+  { simpl trans_state.
     repeat step.
-    edestruct thing as (target & Htarget1 & Htarget2); eauto.
-    epose proof (append_stack_stable_star _ _ Htarget1 (trans_conts kappa)).
-    epose proof (append_stack_stable_star _ _ Htarget2 (trans_conts kappa)).
-    eexists; eauto.
+    assert (Hty: exists T', jt_state GGamma Gamma (mode_eval (trans th) [] (List.map trans_value sigma)) (T')). { admit. }
+
+    unpack.
+
+    pose proof (correctness.correctness_technical _ _ _ _ Hty); unpack.
+
+    eapply star_step_right.
+    {
+      rewrite append_stack_nil_eval.
+      eapply append_stack_stable_star.
+      eauto.
+    }
+  
+    eapply star_step_left.
+    {
+      rewrite append_stack_nil_eval.
+      eapply append_stack_stable_star.
+      eapply thing.
+      eauto. 
+    }
+    simpl.
+    repeat step.
+    repeat eexists; eapply star_refl_eq; eauto; repeat f_equal.
+    pose proof (star_cred_last _ _ H); simpl in *; eauto.
   }
   { eexists; split; asimpl; [|eapply star_refl].
     eapply star_step; [econstructor|]. { eapply trans_value_op_correct; eauto. }
     eapply star_refl.
   }
   Fail next goal.
-Qed.
+Admitted.
 
