theories/typing.v
@@ -523,7 +523,7 @@ In
     { repeat econs_inv; admit. }
     { repeat econs_inv; admit. }
     { repeat econs_inv; admit. }
-  Admitted.
+  Abort.
 
   (* (λ t. < t () | true :- pure 5>) (λ x. Ø) *)
   Example negative_1: ~ jt_term (fun _ => None) [] (App (Lam ((Default [App (Var 0) (Value (VUnit))] (Value (Bool true)) (DefaultPure (Value (Int 5)))))) (Lam Empty)) (TDefault TInteger).
@@ -634,7 +634,7 @@ Module correctness.
   Parameter measure: state -> nat.
   Parameter measure_decrease: forall s1 s2, cred s1 s2 -> measure s2 < measure s1.
 
-  Theorem correctness_technical s1:
+  Theorem correctness_technical_aux s1:
     forall Delta Gamma T,
       jt_state Delta Gamma s1 T ->
       exists s2,
@@ -657,6 +657,28 @@ Module correctness.
     Fail next goal.
   Qed.
 
+  Theorem correctness_technical s1:
+    forall Delta Gamma T,
+      jt_state Delta Gamma s1 T ->
+      exists r sigma,
+        star cred s1 (mode_cont [] sigma r)
+      .
+  Proof.
+    induction s1 using (Wf_nat.induction_ltof1 _ measure).
+    unfold Wf_nat.ltof in H.
+    intros ? ? ? HT.
+    destruct (progress _ _ _ _ HT).
+    * unpack.
+      edestruct (H s2).
+      { eapply measure_decrease; eauto. }
+      { eapply preservation; eauto. }
+      { unpack. eexists; eauto with sequences. }
+    * unpack.
+      induction s1; simpl in *; subst; inj.
+      repeat eexists; eapply star_refl; eauto.
+    Fail next goal.
+  Qed.
+
 
   Theorem correctness:
     forall Delta t T,
@@ -669,7 +691,7 @@ Module correctness.
   .
   Proof.
     intros.
-    destruct correctness_technical with
+    destruct correctness_technical_aux with
       (mode_eval t [] [])
       Delta
       ([]: list type)
